## Angelic Statement
```Lean
intro hn; subst hn
```
## Residual State
```Lean
1 goal

hn : 3 > 0
h_base_case_n1 : 3 = 1 →
  ∑ r ∈ Finset.Icc 0 ((3 - 1) / 2), ((↑3 - 2 * ↑r) * ↑(Nat.choose 3 r) / ↑3) ^ 2 = ↑((2 * 3 - 2).choose (3 - 1)) / ↑3
h_base_case_n2 : 3 = 2 →
  ∑ r ∈ Finset.Icc 0 ((3 - 1) / 2), ((↑3 - 2 * ↑r) * ↑(Nat.choose 3 r) / ↑3) ^ 2 = ↑((2 * 3 - 2).choose (3 - 1)) / ↑3
⊢ ∑ r ∈ Finset.Icc 0 ((3 - 1) / 2), ((↑3 - 2 * ↑r) * ↑(Nat.choose 3 r) / ↑3) ^ 2 = ↑((2 * 3 - 2).choose (3 - 1)) / ↑3
```
## Question 1
<strong><u>Assumptions:</u></strong>
- $3 > 0$.
- If $3 = 1$, then
  $$
  \sum_{r=0}^{\left\lfloor \frac{3-1}{2} \right\rfloor} \left( \frac{3 - 2r}{3} \cdot {3 \choose r} \right)^2 = \frac{{2 \times 3 - 2 \choose 3-1}}{3}
  $$
- If $3 = 2$, then
  $$
  \sum_{r=0}^{\left\lfloor \frac{3-1}{2} \right\rfloor} \left( \frac{3 - 2r}{3} \cdot {3 \choose r} \right)^2 = \frac{{2 \times 3 - 2 \choose 3-1}}{3}
  $$
<strong><u>Goal:</u></strong>
Prove that
$$
\sum_{r=0}^{\left\lfloor \frac{3-1}{2} \right\rfloor} \left( \frac{3 - 2r}{3} \cdot {3 \choose r} \right)^2 = \frac{{2 \times 3 - 2 \choose 3-1}}{3}
$$
## Question 1 (CN)
<strong><u>已知：</u></strong>
- $3 > 0$。
- 若 $3 = 1$，则
  $$
  \sum_{r=0}^{\left\lfloor \frac{3-1}{2} \right\rfloor} \left( \frac{3 - 2r}{3} \cdot {3 \choose r} \right)^2 = \frac{{2 \times 3 - 2 \choose 3-1}}{3}
  $$
- 若 $3 = 2$，则
  $$
  \sum_{r=0}^{\left\lfloor \frac{3-1}{2} \right\rfloor} \left( \frac{3 - 2r}{3} \cdot {3 \choose r} \right)^2 = \frac{{2 \times 3 - 2 \choose 3-1}}{3}
  $$
<strong><u>目标：</u></strong>
证明：
$$
\sum_{r=0}^{\left\lfloor \frac{3-1}{2} \right\rfloor} \left( \frac{3 - 2r}{3} \cdot {3 \choose r} \right)^2 = \frac{{2 \times 3 - 2 \choose 3-1}}{3}
$$